\section{Perturbative expansion in the interaction picture}
Differentiating \( U_s^\dagger \), and noting that \( U_s \) satisfies
\[
\frac{d}{ds} U_s = \frac{i}{\hbar} H_s U_s \quad \Rightarrow \quad \frac{d}{ds} U_s^\dagger = \frac{i}{\hbar} U_s^\dagger H_s \quad \Rightarrow \quad 
dU_s^\dagger = \frac{i}{\hbar} U_s^\dagger H_s \, ds
\]
we substitute into the expression for \( d\ket{\phi_s} \):
\begin{align}
d \ket{\phi_s} 
&= \frac{i}{\hbar} U_s^\dagger H_s \ket{\psi_s} \, ds + U_s^\dagger d \ket{\psi_s} \notag \\
&= \frac{i}{\hbar} U_s^\dagger H_s \ket{\psi_s} \, ds 
+ U_s^\dagger \Bigg[ 
    -\frac{i}{\hbar} H_s \ket{\psi_s} \, ds 
    \\
&\hspace{4em}+ \sum_k i \epsilon L_k \, dW_{k,s} \ket{\psi_s} \notag 
    - \sum_k \frac{\epsilon^2}{2} L_k^\dagger L_k \ket{\psi_s} \, ds 
\Bigg] \notag 
\label{eq:ito_transformed}
\end{align}


The first two terms cancel, yielding:
\begin{equation}
d\ket{\phi_s} = \sum_k \left( i \epsilon \, dW_{k,s} \, U_s^\dagger L_k \ket{\psi_s} 
- \frac{\epsilon^2}{2} \, ds \, U_s^\dagger L_k^\dagger L_k \ket{\psi_s} \right).
\end{equation}

\section{Limit of $\mathcal{C}_M$}
\begin{align}
    [B_m, B_n] &= i^2 \left\{ \sum_{k=1}^{N^2 - 1} L_{k, \frac{m}{M}}\int_\frac{m}{M}^\frac{m+1}{M} dW_{k, \frac{m}{M}}\right\} \left\{ \sum_{l=1}^{N^2 - 1} L_{l, \frac{n}{M}}\int_\frac{n}{M}^\frac{n+1}{M} dW_{l, \frac{n}{M}}\right\} \notag\\
    &-\left\{ \sum_{l=1}^{N^2 - 1} L_{l, \frac{n}{M}}\int_\frac{n}{M}^\frac{n+1}{M} dW_{l, \frac{n}{M}}\right\}\left\{ \sum_{k=1}^{N^2 - 1} L_{k, \frac{m}{M}}\int_\frac{m}{M}^\frac{m+1}{M} dW_{k, \frac{m}{M}}\right\} \notag\\
    &= - \left\{ \sum_{k,l}^{N^2 - 1} \int_\frac{m}{M}^\frac{m+1}{M} dW_{k, \frac{m}{M}} \int_\frac{n}{M}^\frac{n+1}{M} dW_{l, \frac{n}{M}} [L_{k, \frac{m}{M}}, L_{l, \frac{n}{M}}] \right\} \notag\\
    &= - \left\{ \sum_{k,l}^{N^2 - 1} \int_{s_m}^{s_{m+1}} dW_{k,s_m} \int_{s_n}^{s_{n+1}} dW_{l, s_n} [L_{k, s_m}, L_{l, s_n}] \right\}\\
    \mathcal{C}_M &= \sum_{m=0}^{M-1} \sum_{n=0}^{m} [B_m, B_n] \notag\\
    &= - \sum_{m=0}^{M-1} \sum_{n=0}^{m}\left\{ \sum_{k,l}^{N^2 - 1} \int_{s_m}^{s_{m+1}} dW_{k,s_m} \int_{s_n}^{s_{n+1}} dW_{l, s_n} [L_{k, s_m}, L_{l, s_n}] \right\}\\
    \lim_{M\rightarrow\infty}\mathcal{C}_M &= - \sum_{k,l}^{N^2 - 1} \int_{0}^{1} dW_{k,s} \int_{0}^{s} dW_{l, s'} [L_{k, s}, L_{l, s'}] 
\end{align}